From40To50/Call.v
@@ -1,0 +1,697 @@
+From Coq Require Import String ZArith NArith Lia PropExtensionality.
+
+From Vyper Require Import Config Calldag Logic2 Range.
+From Vyper.CheckArith Require Import Builtins.
+From Vyper.L40 Require AST.
+From Vyper.L50 Require AST Call.
+From Vyper.L50 Require Import Types Builtins DynError.
+From Vyper.L10 Require Import Base.
+
+From Vyper.L40Metered Require Import Interpret.
+
+From Vyper.From40To50 Require Import Translate Proto Mangle Expr Stmt.
+
+
+Local Definition OnlyVars {C: VyperConfig}
+                          (loc: string_map dynamic_value)
+: Prop
+:= forall (name: string)
+          (H: map_lookup loc name <> None),
+   exists k, make_var_name "var" k = name.
+
+Local Lemma only_vars_empty {C: VyperConfig}:
+  let _ := string_map_impl in OnlyVars Map.empty.
+Proof.
+cbn. intros name H.
+exfalso.
+exact (H (Map.empty_lookup name)).
+Qed.
+
+(*
+Local Lemma var_finder_empty {C: VyperConfig}:
+  let _ := string_map_impl in VarFinder Map.empty 0%N.
+*)
+
+Local Lemma only_vars_insert {C: VyperConfig}
+                              (loc: string_map dynamic_value)
+                              (key: N)
+                              (value: dynamic_value)
+                              (F: OnlyVars loc):
+  OnlyVars (map_insert loc (make_var_name "var" key) value).
+Proof.
+intros name H.
+unfold map_lookup in H. unfold map_insert in H. rewrite Map.insert_ok in H.
+destruct string_dec as [E|NE].
+{ exists key. exact E. }
+exact (F name H).
+Qed.
+
+(*
+Local Lemma var_finder_insert {C: VyperConfig}
+                              (loc: string_map dynamic_value)
+                              (bound key: N)
+                              (value: dynamic_value)
+                              (F: VarFinder loc bound):
+  VarFinder (map_insert loc (make_var_name "var" key) value) (N.max bound (N.succ key)).
+Proof.
+intros name H.
+unfold map_lookup in H. unfold map_insert in H. rewrite Map.insert_ok in H.
+destruct string_dec as [E|NE].
+{ exists key.  split. { lia. } exact E. }
+destruct (F name H) as (f, OkF).
+exists f. split. { lia. } tauto.
+Qed.
+*)
+
+Local Definition bind_args {C: VyperConfig}
+                           (args: list uint256)
+                           (arity start: N)
+                           (loc: string_map dynamic_value)
+:= LocalVars.bind_vars_to_values 
+     (List.map (fun n : N => (U256, make_var_name "var" n)) (range start arity))
+     (List.map (fun x : uint256 => existT _ U256 (yul_uint256 x))
+         args) loc.
+
+Definition ArgsAgree {C: VyperConfig}
+                     (args: list uint256)
+                     (loc: string_map dynamic_value)
+:= OnlyVars loc
+    /\
+   forall k,
+     option_map (fun x : uint256 => existT _ U256 (yul_uint256 x))
+                (List.nth_error args (N.to_nat k))
+      =
+     map_lookup loc (make_var_name "var" k).
+
+Lemma args_agree_nil {C: VyperConfig}:
+  let _ := string_map_impl in
+  ArgsAgree nil Map.empty.
+Proof.
+split. { apply only_vars_empty. }
+unfold map_lookup. intro k. rewrite Map.empty_lookup.
+rewrite (proj2 (List.nth_error_None _ _)). { easy. }
+cbn. lia.
+Qed.
+
+Definition bind_args_ok {C: VyperConfig}
+                        (args prefix: list uint256)
+                        (arity: N)
+                        (loc: string_map dynamic_value)
+                        (F: ArgsAgree prefix loc):
+  let b := bind_args args arity (N.of_nat (List.length prefix)) loc in
+  match (List.length args ?= N.to_nat arity) with
+  | Lt => b = inl DE_TooFewValues
+  | Gt => b = inl DE_TooManyValues
+  | Eq => match b with
+          | inl _ => False
+          | inr result => ArgsAgree (prefix ++ args) result
+          end
+  end.
+Proof.
+unfold ArgsAgree in *.
+remember (N.to_nat arity) as n.
+unfold bind_args. rewrite range_via_nat.
+remember (make_var_name "var") as var_name.
+revert prefix arity Heqn args loc F. induction n; intros; rewrite<- Heqn.
+{
+  destruct args as [|h]; cbn. 2:trivial.
+  rewrite List.app_nil_r. exact F.
+}
+destruct args as [|h]; cbn. { trivial. }
+assert (OkN: n = N.to_nat (N.pred arity)) by lia.
+repeat rewrite Nat2N.id.
+assert (X: forall x, x + S n - 1 - n = x) by lia. repeat rewrite X. clear X.
+assert (M: map_lookup loc (var_name (N.of_nat (Datatypes.length prefix))) = None).
+{
+  rewrite<- (proj2 F).
+  enough (A: List.nth_error prefix (N.to_nat (N.of_nat (Datatypes.length prefix))) = None)
+    by now rewrite A.
+  apply List.nth_error_None.
+  lia.
+}
+rewrite M.
+assert (IH := IHn (prefix ++ h :: nil)%list (N.pred arity) OkN args
+                  ((map_insert loc (var_name (N.of_nat (Datatypes.length prefix)))
+                               (existT (fun t : yul_type => yul_value t) U256 (yul_uint256 h))))).
+cbn. cbn in IH.
+unfold range_nat in IH.
+subst n.
+repeat rewrite<- List.app_assoc in IH. cbn in IH.
+repeat rewrite List.app_length in IH. cbn in IH.
+repeat rewrite Nat2N.id in *.
+assert (R: forall x y, x + 1 + y = x + S y) by lia. repeat rewrite R in IH.
+apply IH. clear IH IHn R.
+split.
+{
+  subst var_name.
+  apply only_vars_insert.
+  tauto.
+}
+intro k.
+unfold map_lookup. unfold map_insert. rewrite Map.insert_ok.
+destruct string_dec as [E|NE].
+{
+  subst var_name. apply make_var_name_inj in E.
+  subst k. rewrite Nat2N.id.
+  rewrite List.nth_error_app2 by lia.
+  now rewrite Nat.sub_diag.
+}
+assert (K := proj2 F k).
+assert (T := N.lt_trichotomy k (N.of_nat (Datatypes.length prefix))).
+destruct T as [LT | [EQ | GT]].
+{
+  rewrite List.nth_error_app1 by lia.
+  apply K.
+}
+{ subst k. contradiction. }
+rewrite (proj2 (List.nth_error_None _ _)). 2:{ rewrite List.app_length. cbn. lia. }
+rewrite (proj2 (List.nth_error_None _ _)) in K. 2:{ lia. }
+apply K.
+Qed.
+
+Fixpoint bind_zeros {C: VyperConfig}
+                    (loc: string_map dynamic_value)
+                    (start: N)
+                    (count: nat)
+{struct count}
+:= match count with
+   | O => loc
+   | S count' => bind_zeros (map_insert loc (make_var_name "var" start)
+                                            (existT _ U256 (yul_uint256 zero256)))
+                            (N.succ start)
+                            count'
+   end.
+
+Definition lookup_in_init_loc {C: VyperConfig} (args: list uint256) (cap: N) (index: N)
+: option dynamic_value
+:= if (index <? N.max cap (N.of_nat (List.length args)))%N
+     then Some (existT _ U256 (yul_uint256 (List.nth (N.to_nat index) args zero256)))
+     else None.
+
+Definition ArgsAndZerosAgree {C: VyperConfig}
+                             (loc: string_map dynamic_value)
+                             (args: list uint256)
+                             (cap: N)
+:= (forall name, map_lookup loc name <> None ->
+      name = "$$result"%string \/ exists k : N, make_var_name "var" k = name)
+     /\
+    map_lookup loc "$$result" = Some (existT _ U256 (yul_uint256 zero256))
+     /\
+    forall k, map_lookup loc (make_var_name "var" k) = lookup_in_init_loc args cap k.
+
+Lemma zeros_eq {C: VyperConfig}:
+  int_zero_value I256 false = yul_uint256 zero256.
+Proof.
+unfold int_zero_value.
+unfold zero256.
+unfold yul_uint256.
+f_equal.
+apply Eqdep_dec.eq_proofs_unicity.
+decide equality.
+Qed.
+
+Lemma args_and_zeros_agree_init {C: VyperConfig}
+                                (args: list uint256)
+                                (loc_with_args: string_map dynamic_value)
+                                (A: ArgsAgree args loc_with_args)
+                                (varcap: N)
+                                (SmallVarcap: (varcap <= (N.of_nat (List.length args)))%N):
+  ArgsAndZerosAgree
+     (map_insert loc_with_args "$$result"
+                     (existT _ U256 (int_zero_value I256 false)))
+     args
+     varcap.
+Proof.
+unfold ArgsAndZerosAgree.
+unfold map_lookup. unfold map_insert.
+repeat split; intros; repeat rewrite Map.insert_ok in *.
+{
+  rewrite Map.insert_ok in H.
+  destruct string_dec as [|NE]. { now left. }
+  right. now apply A.
+}
+{
+  destruct string_dec. 2:contradiction.
+  repeat f_equal. apply zeros_eq.
+}
+destruct string_dec. { discriminate. }
+unfold lookup_in_init_loc.
+unfold ArgsAgree in A. unfold map_lookup in A.
+rewrite<- (proj2 A k).
+destruct (Nat.lt_ge_cases (N.to_nat k) (List.length args)) as [KL|KGE].
+{
+  replace ((k <? N.max varcap (N.of_nat (Datatypes.length args)))%N) with true.
+  2:{ symmetry. apply N.ltb_lt. lia. }
+  remember (List.nth_error args (N.to_nat k)) as x. symmetry in Heqx.
+  destruct x as [x|]. 2:{ exfalso. apply (proj2 (List.nth_error_Some _ _) KL Heqx). }
+  now rewrite (List.nth_error_nth _ _ _ Heqx).
+}
+replace ((k <? N.max varcap (N.of_nat (Datatypes.length args)))%N) with false.
+2:{ symmetry. apply N.ltb_ge. lia. }
+now rewrite (proj2 (List.nth_error_None _ _) KGE).
+Qed.
+
+Lemma args_and_zeros_agree_step {C: VyperConfig}
+                                (args: list uint256)
+                                (loc: string_map dynamic_value)
+                                (varcap: N)
+                                (A: ArgsAndZerosAgree loc args varcap)
+                                (LargeVarcap: ((N.of_nat (List.length args)) <= varcap)%N):
+  ArgsAndZerosAgree
+     (map_insert loc (make_var_name "var" varcap)
+                     (existT _ U256 (yul_uint256 zero256)))
+     args
+     (N.succ varcap).
+Proof.
+unfold ArgsAndZerosAgree.
+unfold map_lookup. unfold map_insert.
+repeat split; intros; repeat rewrite Map.insert_ok in *.
+{
+  rewrite Map.insert_ok in H.
+  destruct string_dec as [|NE]. { right. now exists varcap. }
+  now apply A.
+}
+{
+  destruct string_dec. 1:discriminate.
+  apply A.
+}
+destruct string_dec as [E|NE].
+{
+  apply make_var_name_inj in E.
+  subst k.
+  unfold lookup_in_init_loc.
+  replace (varcap <? N.max (N.succ varcap) (N.of_nat (Datatypes.length args)))%N with true.
+  2:{ symmetry. apply N.ltb_lt. lia. }
+  now rewrite List.nth_overflow by lia.
+}
+destruct A as (_, (_, A)).
+unfold map_lookup in A.
+rewrite A.
+unfold lookup_in_init_loc.
+destruct (N.lt_trichotomy k varcap) as [LT|[EQ|GT]].
+{
+  replace (k <? N.max varcap (N.of_nat (Datatypes.length args)))%N with true.
+  2:{ symmetry. apply N.ltb_lt. lia. }
+  replace (k <? N.max (N.succ varcap) (N.of_nat (Datatypes.length args)))%N with true.
+  2:{ symmetry. apply N.ltb_lt. lia. }
+  trivial.
+}
+{ now subst. }
+replace (k <? N.max varcap (N.of_nat (Datatypes.length args)))%N with false.
+2:{ symmetry. apply N.ltb_ge. lia. }
+replace (k <? N.max (N.succ varcap) (N.of_nat (Datatypes.length args)))%N with false.
+2:{ symmetry. apply N.ltb_ge. lia. }
+trivial.
+Qed.
+
+Lemma bind_zeros_ok {C: VyperConfig}
+                    (args: list uint256)
+                    (l: string_map dynamic_value)
+                    (n: nat)
+                    (Init: ArgsAndZerosAgree l args (N.of_nat (Datatypes.length args))):
+  ArgsAndZerosAgree (bind_zeros l (N.of_nat (Datatypes.length args)) n) args
+    (N.of_nat (n + Datatypes.length args)).
+Proof.
+remember n as k. replace k with n at 2.
+replace (N.of_nat (Datatypes.length args)) with (N.of_nat (n - k + Datatypes.length args)) in Init by lia.
+replace (N.of_nat (Datatypes.length args)) with (N.of_nat (n - k + Datatypes.length args)) by lia.
+assert (K: k <= n) by lia.
+clear Heqk.
+revert l Init K. induction k; intros. { now rewrite Nat.sub_0_r in Init. }
+simpl.
+assert (G: ArgsAndZerosAgree
+             (map_insert l (make_var_name "var" (N.of_nat (n - S k + Datatypes.length args)))
+                (existT (fun t : yul_type => yul_value t) U256 (yul_uint256 zero256))) args
+             (N.succ (N.of_nat (n - S k + Datatypes.length args)))).
+{
+  apply (args_and_zeros_agree_step _ _ _ Init).
+  lia.
+}
+replace (N.succ (N.of_nat (n - S k + Datatypes.length args)))
+   with (N.of_nat (n - k + Datatypes.length args))
+   in * by lia.
+apply (IHk _ G (le_Sn_le _ _ K)).
+Qed.
+
+Lemma bind_zeros_for_loc_with_args {C: VyperConfig}
+                                   (args: list uint256)
+                                   (loc_with_args: string_map dynamic_value)
+                                   (A: ArgsAgree args loc_with_args)
+                                   (varcap: N):
+  ArgsAndZerosAgree
+    (bind_zeros (map_insert loc_with_args "$$result"
+                           (existT _ U256 (int_zero_value I256 false)))
+                     (N.of_nat (List.length args))
+                     (N.to_nat varcap - List.length args))
+    args varcap.
+Proof.
+destruct (Nat.lt_ge_cases (N.to_nat varcap) (List.length args)) as [L|GE].
+{ (* small varcap *)
+  replace (N.to_nat varcap - Datatypes.length args) with 0 by lia.
+  cbn.
+  apply (args_and_zeros_agree_init args loc_with_args A). lia.
+}
+remember (N.to_nat varcap - List.length args) as n.
+assert (V: varcap = N.of_nat (n + List.length args)) by lia.
+subst varcap.
+clear Heqn GE.
+assert (Init := args_and_zeros_agree_init _ _ A (N.of_nat (Datatypes.length args)) (N.le_refl _)).
+remember (map_insert loc_with_args "$$result"
+            (existT _ U256 (int_zero_value I256 false))) as l. clear Heql. clear A.
+now apply bind_zeros_ok.
+Qed.
+
+
+Local Lemma interpret_generated_var_decls {C: VyperConfig}
+                                          (max_loop_iterations: nat)
+                                          (builtins50: string -> option L50.Builtins.yul_builtin)
+                                          (decls50: string_map L50.AST.fun_decl)
+                                          (this_fun_decl50: option L50.AST.fun_decl)
+                                          (args: list uint256)
+                                          (loc: string_map dynamic_value)
+                                          (arity varcap: N)
+                                          (ArityOk: arity = N.of_nat (List.length args))
+                                          (A: ArgsAndZerosAgree loc args arity)
+                                          (call50: L50.AST.fun_decl -> world_state -> list dynamic_value ->
+                                                   world_state * option (expr_result (list dynamic_value)))
+                                          (world: world_state):
+   L50.Stmt.interpret_stmt_list_no_unbind max_loop_iterations builtins50 (map_lookup decls50)
+     this_fun_decl50 call50
+     world loc
+     (make_var_declarations arity varcap)
+    =
+   (world,
+    bind_zeros loc arity (N.to_nat (varcap - arity)%N),
+    Some StmtSuccess,
+    List.map (fun k => (U256, make_var_name "var" k))
+             (List.rev (range arity (varcap - arity)%N))).
+Proof.
+unfold make_var_declarations.
+rewrite range_via_nat.
+remember (N.to_nat (varcap - arity)%N) as n.
+clear varcap Heqn.
+subst arity.
+remember n as k.
+replace (N.of_nat (Datatypes.length args)) with (N.of_nat (n - k + Datatypes.length args)) in A by lia.
+replace (N.of_nat (Datatypes.length args)) with (N.of_nat (n - k + Datatypes.length args)) by lia.
+assert (K: k <= n) by lia.
+clear Heqk.
+revert loc K A. induction k; intros. { easy. }
+simpl.
+rewrite Nat2N.id.
+replace (n - S k + Datatypes.length args + S k - 1 - k) with (n - S k + Datatypes.length args) by lia.
+
+(* shadowing check *)
+rewrite (proj2 (proj2 A) (N.of_nat (n - S k + Datatypes.length args))).
+unfold lookup_in_init_loc.
+replace (N.of_nat (n - S k + Datatypes.length args) <?
+         N.max (N.of_nat (n - S k + Datatypes.length args)) (N.of_nat (Datatypes.length args)))%N
+  with false by (symmetry; apply N.ltb_ge; lia).
+assert (G: ArgsAndZerosAgree
+             (map_insert loc (make_var_name "var" (N.of_nat (n - S k + Datatypes.length args)))
+                (existT (fun t : yul_type => yul_value t) U256 (int_zero_value I256 false))) args (N.of_nat (n - k + Datatypes.length args))).
+{
+  replace (N.of_nat (n - k + Datatypes.length args))
+    with (N.succ (N.of_nat (n - S k + Datatypes.length args))) by lia.
+  rewrite zeros_eq.
+  apply (args_and_zeros_agree_step _ _ _ A).
+  lia.
+}
+assert (IH := IHk (map_insert loc (make_var_name "var" (N.of_nat (n - S k + Datatypes.length args)))
+                  (existT (fun t : yul_type => yul_value t) U256 (int_zero_value I256 false)))
+                  (le_Sn_le _ _ K) G).
+replace (n - S k + Datatypes.length args + S k - 1) with (n - k + Datatypes.length args + k - 1) by lia.
+unfold range_nat in IH.
+rewrite Nat2N.id in IH.
+rewrite IH.
+f_equal. 2:{ now rewrite List.map_app. }
+repeat f_equal; trivial. { apply zeros_eq. }
+lia.
+Qed.
+
+
+Lemma interpret_translated_call {C: VyperConfig}
+                                (max_call_depth: nat)
+                                (max_loop_iterations: nat)
+
+                                {B: builtin_names_config}
+                                (builtins40: string -> option L10.Base.builtin)
+                                (builtins50: string -> option L50.Builtins.yul_builtin)
+                                (BuiltinsOk: AllBuiltinsAgreeIfU256 builtins40 builtins50)
+                                (BuiltinsBasics: BuiltinsSupportBasics builtins50)
+                                (BuiltinsSafe: forall x,
+                                                 builtins50 ("$" ++ x)%string = None)
+                                (BuiltinsHaveArith: BuiltinsSupportUInt256 B builtins40)
+
+                                {protos: string_map proto}
+                                (KnownProtosOk: check_known_protos B (map_lookup protos) = true)
+                                (ProtosOk: ProtosAgree (map_lookup protos) builtins50)
+
+                                {decls40: string_map L40.AST.decl}
+                                {decls50: string_map L50.AST.fun_decl}
+                                (DeclsOk: translate_fun_decls B protos decls40 = inr decls50)
+
+                                (d40: L40.AST.decl)
+                                (d50: L50.AST.fun_decl)
+                                (Ok: translate_fun_decl B protos d40 = inr d50)
+
+                                (EnoughIterationsForEverything:
+                                   (L40.AST.max_loop_count_decl_map decls40 < N.of_nat max_loop_iterations)%N)
+                                (EnoughIterations:
+                                   (L40.AST.max_loop_count_decl d40 < N.of_nat max_loop_iterations)%N)
+
+                                (world: world_state)
+                                (arg_values: list uint256):
+  ResultsAgree
+    (interpret_call_metered max_call_depth decls40 builtins40 d40 world arg_values)
+    (L50.Call.interpret_call max_call_depth max_loop_iterations builtins50
+                             (map_lookup decls50) d50 world
+                             (List.map (fun x => (existT _ U256 (yul_uint256 x))) arg_values))
+    1%N.
+Proof.
+revert max_loop_iterations d40 d50 Ok world arg_values EnoughIterations EnoughIterationsForEverything.
+induction max_call_depth; intros. { easy. }
+cbn.
+pose (decl40 := d40).
+pose (decl50 := d50).
+assert (Ok': translate_fun_decl B protos decl40 = inr decl50) by assumption.
+destruct d40 as (fn_name, arity40, body40).
+cbn in Ok.
+remember (translate_block true B protos body40 0) as body. symmetry in Heqbody.
+destruct body as [|(body50)]. { discriminate. } (* body50 is executed after the var decls *)
+inversion Ok. subst d50. clear Ok.
+remember interpret_block_metered as do_block40.  (* saving from cbn *)
+remember L50.Stmt.interpret_block as do_block50.
+remember LocalVars.get_vars_by_typenames as get_output.
+cbn.
+
+remember (LocalVars.bind_vars_to_values (make_input_typenames arity40)
+            (List.map (fun x : uint256 => existT (fun t : yul_type => yul_value t) U256 (yul_uint256 x))
+                arg_values) Map.empty) as loc_with_args.
+assert (ViaBindArgs: let _ := string_map_impl in
+                     loc_with_args = bind_args arg_values arity40 0 Map.empty)
+  by easy.
+cbn in ViaBindArgs.
+assert (BA := bind_args_ok arg_values nil arity40 _ args_agree_nil).
+cbn in BA.
+repeat rewrite<- ViaBindArgs in BA.
+remember (Datatypes.length arg_values ?= N.to_nat arity40) as cmp. symmetry in Heqcmp.
+destruct cmp.
+2:{
+  apply nat_compare_Lt_lt in Heqcmp.
+  assert (NE: Datatypes.length arg_values =? N.to_nat arity40 = false).
+  { apply Nat.eqb_neq. lia. }
+  rewrite NE. rewrite BA. cbn.
+  replace (match N.to_nat arity40 with
+           | 0 => false
+           | S m' => Datatypes.length arg_values <=? m'
+           end) with (Datatypes.length arg_values <? N.to_nat arity40) by easy.
+  rewrite (proj2 (Nat.ltb_lt _ _) Heqcmp).
+  easy.
+}
+2:{
+  apply nat_compare_Gt_gt in Heqcmp. apply gt_not_le in Heqcmp. apply not_le in Heqcmp.
+  assert (NE: Datatypes.length arg_values =? N.to_nat arity40 = false).
+  { apply Nat.eqb_neq. lia. }
+  rewrite NE. rewrite BA. cbn.
+  replace (match N.to_nat arity40 with
+           | 0 => false
+           | S m' => Datatypes.length arg_values <=? m'
+           end) with (Datatypes.length arg_values <? N.to_nat arity40) by easy.
+  assert (Q: Datatypes.length arg_values <? N.to_nat arity40 = false) by (rewrite Nat.ltb_ge; lia).
+  now rewrite Q.
+}
+apply Nat.compare_eq in Heqcmp.
+rewrite (proj2 (Nat.eqb_eq _ _) Heqcmp).
+destruct loc_with_args as [|loc_with_args]; try contradiction.
+
+assert (ResultUndeclared: map_lookup loc_with_args "$$result" = None).
+{
+  destruct BA as (OV, _).
+  assert (OVR := OV "$$result"%string).
+  destruct (map_lookup loc_with_args "$$result"). 2:{ trivial. }
+  assert (D: Some d <> None) by discriminate.
+  destruct (OVR D) as (k, X).
+  discriminate.
+}
+rewrite ResultUndeclared.
+subst do_block50.
+rewrite L50.Stmt.interpret_stmt_list_ok.
+rewrite L50.Stmt.interpret_stmt_list_unbind_later.
+rewrite L50.Stmt.interpret_stmt_list_no_unbind_app.
+
+assert (AInit := args_and_zeros_agree_init _ _ BA _ (N.le_refl _)).
+assert (Arity40Ok: arity40 = N.of_nat (Datatypes.length arg_values)) by lia.
+rewrite<- Arity40Ok in AInit.
+rewrite (interpret_generated_var_decls max_loop_iterations builtins50 decls50
+                                       _ _ _ _ (AST.var_cap_block body40) Arity40Ok AInit _ world).
+
+(* variable declarations done, now there's the post-body assignment that we need to separate *)
+assert (NoVars50: L50.Stmt.stmt_list_has_top_level_var_decls body50 = false)
+  by apply (translated_block_declares_nothing Heqbody).
+assert (NoVarsAssign:
+  Stmt.stmt_list_has_top_level_var_decls
+    (AST.Assign ("$$result"%string :: nil) (AST.Const U256 (yul_uint256 zero256)) :: nil) = false)
+  by easy.
+rewrite L50.Stmt.interpret_stmt_list_no_vars_bind.
+2:{
+  rewrite L50.Stmt.stmt_list_has_top_level_var_decls_app.
+  now rewrite NoVars50.
+}
+rewrite L50.Stmt.interpret_stmt_list_app; try assumption.
+
+(* now we'll look into the variables in pre-body state *)
+assert (PreLocAZ := bind_zeros_for_loc_with_args arg_values loc_with_args BA (AST.var_cap_block body40)).
+replace (N.to_nat (AST.var_cap_block body40) - Datatypes.length arg_values)
+  with (N.to_nat (AST.var_cap_block body40 - arity40))
+  in PreLocAZ by lia.
+rewrite<- Arity40Ok in PreLocAZ.
+remember (bind_zeros
+           (map_insert loc_with_args "$$result"
+              (existT (fun t : yul_type => yul_value t) U256 (int_zero_value I256 false))) arity40
+           (N.to_nat (AST.var_cap_block body40 - arity40)))
+  as pre_loc50.
+clear Heqpre_loc50. (* PreLocAZ should contain everything we need *)
+
+assert (PreLVA: let _ := memory_impl in
+                LocalVarsAgree (OpenArray.from_list arg_values) pre_loc50 (AST.var_cap_block body40)).
+{
+  cbn. intros k L. rewrite OpenArray.from_list_ok.
+  rewrite ((proj2 (proj2 PreLocAZ)) k).
+  unfold lookup_in_init_loc.
+  replace (k <? N.max (AST.var_cap_block body40) (N.of_nat (Datatypes.length arg_values)))%N
+    with true
+    by (symmetry; apply N.ltb_lt; lia).
+  easy.
+}
+assert (PreSV: SecondaryVarsOk nil pre_loc50).
+{
+  split.
+  { now rewrite (proj1 (proj2 PreLocAZ)). }
+  { intros k L. cbn in L. lia. }
+  { intros k L. cbn in L. lia. }
+  {
+    intros k _.
+    assert (P := proj1 PreLocAZ (make_var_name "offset" (N.of_nat k))).
+    destruct (map_lookup pre_loc50 (make_var_name "offset" (N.of_nat k))) as [m|]. 2:trivial.
+    assert (M: Some m <> None) by discriminate.
+    now destruct (P M) as [R|(v, V)].
+  }
+  intros k _.
+  assert (P := proj1 PreLocAZ (make_var_name "cursor" (N.of_nat k))).
+  destruct (map_lookup pre_loc50 (make_var_name "cursor" (N.of_nat k))) as [m|]. 2:trivial.
+  assert (M: Some m <> None) by discriminate.
+  now destruct (P M) as [R|(v, V)].
+}
+
+(* finally it's interpret_translated_block time *)
+subst do_block40.
+remember (interpret_block_metered decls40 (interpret_call_metered max_call_depth decls40 builtins40)
+              builtins40 world (OpenArray.from_list arg_values) nil body40) as output40.
+remember (Stmt.interpret_stmt_list max_loop_iterations builtins50 (map_lookup decls50)
+          _
+          (Call.interpret_call max_call_depth max_loop_iterations builtins50 (map_lookup decls50)) world
+          pre_loc50 body50) as output50.
+
+assert (BodyOk:
+  let '(w, l, result) := output50 in
+  StmtResultsAgree
+    output40
+    (w, l, result)
+    (AST.var_cap_block body40)
+   /\
+  SecondaryVarsOk nil l).
+{
+  subst output40 output50.
+  assert (this_fun40 := L40.AST.FunDecl fn_name arity40 body40).
+
+  assert (LoopDepthOk: @List.length L40.Expr.loop_ctx nil = N.to_nat 0%N) by easy.
+  refine (interpret_translated_block
+                  decls40 decls50 (Some decl40) (Some decl50) Ok' DeclsOk
+    (* call40: *) (interpret_call_metered max_call_depth decls40 builtins40)
+    (* call50: *) (fun m => L50.Call.interpret_call max_call_depth m builtins50 (map_lookup decls50))
+    (* CallsOk *) _
+                  builtins40 builtins50 BuiltinsOk BuiltinsBasics BuiltinsSafe BuiltinsHaveArith
+                  ProtosOk KnownProtosOk world (OpenArray.from_list arg_values) pre_loc50
+                  nil LoopDepthOk PreSV body40 body50 Heqbody
+                  (L40.AST.var_cap_block body40) (N.le_refl _)
+                  PreLVA EnoughIterationsForEverything EnoughIterations).
+  intros max_loop_iterations' d40' d50' dOk' world' args' arity50 Arity50Ok.
+  subst arity50.
+  apply (IHmax_call_depth max_loop_iterations' d40' d50' dOk' world' args').
+}
+clear Heqoutput40 Heqoutput50.
+destruct output40 as ((w40, l40), r40).
+destruct output50 as ((w50, l50), r50).
+destruct r40 as [r40|], r50 as [r50|]; cbn in BodyOk; try easy.
+simpl.
+destruct BodyOk as ((PostLVA, Agreement), PostSV).
+assert (RD := sv_result_declared PostSV).
+destruct (map_lookup l50 "$$result") as [(result_type, _)|]. 2:contradiction.
+destruct (yul_type_eq_dec result_type U256) as [|NE].
+2:{
+  destruct result_type; try contradiction.
+  destruct size; try contradiction.
+  destruct signed; contradiction.
+}
+(* undoing all the local declarations can't undeclare $$result *)
+assert (GetOutput: forall (indices: list N),
+  get_output ((U256, "$$result"%string) :: nil)%list
+      (LocalVars.unbind_vars
+         (List.map (fun k : N => (U256, make_var_name "var" k)) indices)
+         (map_insert l50 "$$result"
+            (existT _ U256 (yul_uint256 zero256))))
+   =
+  inr ((existT _ U256 (yul_uint256 zero256)) :: nil)%list).
+{
+  intro indices.
+  remember (map_insert l50 "$$result"
+             (existT _ U256 (yul_uint256 zero256))) as m.
+  assert (M: map_lookup m "$$result"
+              =
+             Some (existT _ U256 (yul_uint256 zero256))).
+  { subst. unfold map_lookup. unfold map_insert. rewrite Map.insert_ok. now destruct string_dec. }
+  clear Heqm.
+  subst get_output.
+  unfold LocalVars.get_vars_by_typenames.
+  enough (L: map_lookup
+               (LocalVars.unbind_vars (List.map (fun k : N => (U256, make_var_name "var" k)) indices) m)
+               "$$result"
+              =
+             Some (existT _ U256 (yul_uint256 zero256))).
+  { now rewrite L. }
+  unfold map_lookup in *.
+  revert m M. induction indices; intros. { easy. }
+  simpl.
+  apply IHindices.
+  unfold map_remove.
+  rewrite Map.remove_ok.
+  destruct string_dec. { discriminate. }
+  exact M.
+}
+destruct r40 as [|ab40|x40], r50 as [|ab50|x50]; try easy; try rewrite GetOutput;
+  try destruct ab40; try destruct ab50; try easy.
+(* success on both sides *)
+split. { tauto. }
+now rewrite (proj2 Agreement).
+Qed.
